bedrock2/src/BasicC64Semantics.v
@@ -4,14 +4,16 @@ Require bedrock2.String bedrock2.Map.SortedList bedrock2.Map.SortedListString.
 Require Import coqutil.Word.Interface.
 Require coqutil.Word.Naive.
 
+Axiom StrictOrderWord : forall width word, @word.ok width word -> @SortedList.parameters.strict_order (@word.rep _ word) (@word.ltu _ word).
+
+Existing Instance Word.Naive.ok.
 Instance parameters : parameters :=
   let word := Word.Naive.word 64 eq_refl in
   let byte := Word.Naive.word 8 eq_refl in
   {|
   syntax := StringNamesSyntax.make BasicC64Syntax.StringNames_params;
-  mem := SortedList.map (SortedList.parameters.Build_parameters word byte word.eqb word.ltu);
+  mem := SortedList.map (SortedList.parameters.Build_parameters word byte word.ltu) (StrictOrderWord _ _ _);
   locals := SortedListString.map _;
   interp_binop := Basic_bopnames.interp_binop;
   funname_eqb := String.eqb;
 |}.
-Existing Instance Word.Naive.ok.
